interface for Benton2004.SmithVolpano

examples/rel/Benton2004.SmithVolpano.fsti
@@ -14,34 +14,61 @@
    limitations under the License.
 *)
 module Benton2004.SmithVolpano
+include Benton2004.DDCC
 
-let eval_equiv_def
+type seclevel = | Low | High
+
+let interp_seclevel (t: Type0) (s: seclevel) : GTot (nstype t) =
+  match s with
+  | Low -> ns_delta
+  | High -> ns_t
+
+type context = (l: list (var * seclevel) { List.Tot.noRepeats (List.Tot.map fst l) } )
+
+let rec interp_context
+  (gamma: context)
+: Ghost sttype
+  (requires True)
+  (ensures (fun phi -> forall x' . List.Tot.mem x' (List.Tot.map fst gamma) == false ==> x' `st_fresh_in` phi))
+=  match gamma with
+  | [] -> st_nil
+  | (x, s) :: gamma' -> st_cons (interp_context gamma') x (interp_seclevel int s)
+
+let eval_equiv
+  (#t: Type0)
+  (c: context)
+  (f: exp t)
+  (s: seclevel)
+: GTot Type0
+= Benton2004.DDCC.eval_equiv (interp_context c) (interp_seclevel _ s) f f
+
+val eval_equiv_def
   (#t: Type0)
   (gamma: context)
   (f: exp t)
   (s: seclevel)
 : Lemma
   (eval_equiv gamma f s <==> Benton2004.DDCC.eval_equiv (interp_context gamma) (interp_seclevel _ s) f f)
-= ()
 
-let exec_equiv
+val exec_equiv
   (gamma: context)
   (c: computation)
   (s: seclevel)
 : GTot Type0
-= Benton2004.DDCC.exec_equiv (interp_context gamma) (interp_context gamma) c (match s with Low -> c | High -> skip)
 
-let exec_equiv_def
+val exec_equiv_def
   (gamma: context)
   (c: computation)
   (s: seclevel)
 : Lemma
   (exec_equiv gamma c s <==> Benton2004.DDCC.exec_equiv (interp_context gamma) (interp_context gamma) c (match s with Low -> c | High -> skip))
-= ()
 
 (* Figure 4 *)
 
-let eval_equiv_var_same
+let fresh_in (x: var) (gamma: context) : GTot Type0 =
+  List.Tot.mem x (List.Tot.map fst gamma) == false
+
+val eval_equiv_var_same
   (gamma: context)
   (x: var)
   (s: seclevel)
@@ -52,9 +79,8 @@ let eval_equiv_var_same
     eval_equiv ((x, s) :: gamma) (evar x) s
   ))
   [SMTPat (eval_equiv ((x, s)::gamma) (evar x) s)]
-= d_v x (interp_context gamma) (interp_seclevel int s)
 
-let eval_equiv_var_other
+val eval_equiv_var_other
   (gamma: context)
   (x y: var)
   (sx sy: seclevel)
@@ -69,9 +95,8 @@ let eval_equiv_var_other
     eval_equiv ((y, sy) :: gamma) (evar x) sx
   ))
   [SMTPat (eval_equiv ((y, sy)::gamma) (evar x) sx)]
-= ()
 
-let eval_equiv_const
+val eval_equiv_const
   (#t: Type0)
   (gamma: context)
   (c: t)
@@ -79,17 +104,15 @@ let eval_equiv_const
 : Lemma
   (eval_equiv gamma (const c) s)
   [SMTPat (eval_equiv gamma (const c) s)]
-= Benton2004.DDCC.eval_equiv_const c (interp_context gamma)
 
-let op_abs_interp_seclevel
+val op_abs_interp_seclevel
   (#from #to: Type0)
   (op: (from -> from -> Tot to))
   (s: seclevel)
 : Lemma
   (op_abs op (interp_seclevel _ s) (interp_seclevel _ s) (interp_seclevel _ s))
-= ()
 
-let eval_equiv_op
+val eval_equiv_op
   (#from #to: Type0)
   (op: (from -> from -> Tot to))
   (gamma: context)
@@ -102,10 +125,8 @@ let eval_equiv_op
   ))
   (ensures (eval_equiv gamma (eop op e e') s))
   [SMTPat (eval_equiv gamma (eop op e e') s)]  
-= op_abs_interp_seclevel op s;
-  d_op op e e e' e' (interp_seclevel _ s) (interp_seclevel _ s) (interp_seclevel _ s) (interp_context gamma)
 
-let exec_equiv_assign
+val exec_equiv_assign
   (gamma: context)
   (x: var)
   (e: exp int)
@@ -120,11 +141,8 @@ let exec_equiv_assign
     exec_equiv ((x, s)::gamma) (assign x e) s
   ))
   [SMTPat (exec_equiv ((x, s)::gamma) (assign x e) s)]
-= match s with
-  | Low -> d_assign (interp_context gamma) x (interp_seclevel _ s) (interp_seclevel _ s) e e
-  | High -> d_das x e (interp_context gamma) (interp_seclevel _ s) 
 
-let exec_equiv_seq
+val exec_equiv_seq
   (gamma: context)
   (c c' : computation)
   (s: seclevel)
@@ -137,12 +155,8 @@ let exec_equiv_seq
     exec_equiv gamma (seq c c') s
   ))
   [SMTPat (exec_equiv gamma (seq c c') s)]
-= match s with
-  | Low -> ()
-  | High -> d_su1' c c' skip (interp_context gamma) (interp_context gamma) (interp_context gamma) // FIXME: WHY WHY WHY does this pattern NOT trigger?
   
-
-let exec_equiv_ifthenelse
+val exec_equiv_ifthenelse
   (gamma: context)
   (b: exp bool)
   (c c' : computation)
@@ -155,9 +169,8 @@ let exec_equiv_ifthenelse
   ))
   (ensures (exec_equiv gamma (ifthenelse b c c') s))
   [SMTPat (exec_equiv gamma (ifthenelse b c c') s)]
-= ()
 
-let exec_equiv_while
+val exec_equiv_while
   (gamma: context)
   (b: exp bool)
   (c: computation)
@@ -168,9 +181,8 @@ let exec_equiv_while
   ))
   (ensures (exec_equiv gamma (while b c) Low))
   [SMTPat (exec_equiv gamma (while b c) Low)]
-= ()
 
-let eval_equiv_low_to_high
+val eval_equiv_low_to_high
   (#t: Type0)
   (gamma: context)
   (e: exp t)
@@ -178,13 +190,20 @@ let eval_equiv_low_to_high
   (requires (eval_equiv gamma e Low))
   (ensures (eval_equiv gamma e High))
   [SMTPat (eval_equiv gamma e High)]
-= ()
 
-let exec_equiv_high_to_low
+val exec_equiv_high_to_low
   (gamma: context)
   (c: computation)
 : Lemma
   (requires (exec_equiv gamma c High))
   (ensures (exec_equiv gamma c Low))
   [SMTPat (exec_equiv gamma c Low)]
-= ()
+
+(* Definition 2 *)
+
+let strong_sequential_noninterference
+  (gamma: context)
+  (c: computation)
+: GTot Type0
+= exec_equiv gamma c Low
+
